Finished part 1 and started part 2

assignment.v
@@ -2,372 +2,433 @@ Require Import Arith.
 Require Import List.
 Import ListNotations.
 
-Inductive tree : Set :=
-| leaf : tree
-| node : tree -> nat -> tree -> tree.
 
-Fixpoint all_leq(n: nat)(t: tree): Prop :=
-  match t with
+Section TypeAndFunctionDefinitions.
+  Inductive tree : Set :=
+  | leaf : tree
+  | node : tree -> nat -> tree -> tree.
+
+  Fixpoint all_leq(n: nat)(t: tree): Prop :=
+    match t with
+      | leaf => True
+      | node l val r => (val <= n) /\ (all_leq n l) /\ (all_leq n r)
+    end.
+
+  Fixpoint all_geq(n: nat)(t: tree): Prop := 
+    match t with
+      | leaf => True
+      | node l val r => (val > n) /\ (all_geq n l) /\ (all_geq n r)
+    end. 
+
+  Fixpoint bst (T: tree): Prop :=
+    match T with
     | leaf => True
-    | node l val r => (val <= n) /\ (all_leq n l) /\ (all_leq n r)
+    | node l v r => (all_leq v l) /\ (all_geq v r) /\ bst l /\ bst r
   end.
 
-Fixpoint all_geq(n: nat)(t: tree): Prop := 
-  match t with
-    | leaf => True
-    | node l val r => (val > n) /\ (all_geq n l) /\ (all_geq n r)
-  end. 
+  Fixpoint insert(n: nat)(T: tree): tree :=
+    match T with
+    | leaf => node leaf n leaf
+    | node l v r => if n <=? v then node (insert n l) v r else node l v (insert n r)
+    end.
 
-Fixpoint bst (T: tree): Prop :=
-  match T with
-  | leaf => True
-  | node l v r => (all_leq v l) /\ (all_geq v r) /\ bst l /\ bst r
-end.
+  Fixpoint occurs(n: nat)(t: tree): Prop :=
+    match t with
+      | leaf => False
+      | node l v r => v = n \/ occurs n l \/ occurs n r
+    end.
 
-Fixpoint insert(n: nat)(T: tree): tree :=
-  match T with
-  | leaf => node leaf n leaf
-  | node l v r => if n <=? v then node (insert n l) v r else node l v (insert n r)
-  end.
+  Definition occurs_opt(n: option nat)(t: tree): Prop :=
+    match n with
+      | None => False
+      | Some x => occurs x t
+    end.
 
-Fixpoint occurs(n: nat)(t: tree): Prop :=
-  match t with
+  Fixpoint sort_insert(l: list nat): (tree) :=
+    match l with
+    | nil => leaf
+    | cons x xs => insert x (sort_insert xs)
+    end.
+
+  Fixpoint to_list(t: tree): (list nat) :=
+    match t with
+    | leaf => []
+    | node l v r => (to_list l) ++ v::to_list r
+    end.
+
+  Definition sort(t : tree) : tree :=
+    sort_insert (to_list t).
+  
+  Fixpoint list_min(l: list nat) : option nat:=
+    match l with
+    | nil => None
+    | cons x xs => match list_min xs with
+      | None => Some x
+      | Some y => Some (Nat.min x y)
+      end
+    end.
+  
+  Fixpoint treeMin(t: tree): option nat :=
+    match t with
+      | leaf => None
+      | node l v r => 
+        match (treeMin l, treeMin r) with
+          | (None, None) => Some v
+          | (None, Some y) => Some (Nat.min v y)
+          | (Some x, None) => Some (Nat.min v x)
+          | (Some x, Some y) => Some (Nat.min v (Nat.min x y))
+        end
+    end.
+  Print treeMin.
+
+  Fixpoint leftmost(t: tree): option nat :=
+    match t with
+    | leaf => None
+    | node l v r => match leftmost l with
+      | None => Some v
+      | Some y => Some y
+      end
+    end.
+  
+  Fixpoint search(t: tree)(n: nat): Prop :=
+    match t with
     | leaf => False
-    | node l v r => v = n \/ occurs n l \/ occurs n r
-  end.
+    | node l v r => match Nat.compare n v with
+      | Lt => search l n
+      | Eq => True
+      | Gt => search r n
+      end
+    end.
 
-Fixpoint sort_insert(l: (list nat))(t: tree) {struct l}: (tree) :=
-  match l with
-  | nil => t
-  | cons x xs => insert x (sort_insert xs t)
-  end.
+End TypeAndFunctionDefinitions.
 
-Fixpoint to_list(t: tree): (list nat) :=
-  match t with
-  | leaf => []
-  | node l v r => (to_list l) ++ v::to_list r
-  end.
-
-
-Definition sort(t : tree) : tree :=
-  sort_insert (to_list t) leaf.
-
-(* Compute(insert 2 (node leaf 3 leaf)). *)
-
-(*Print Nat.*)
-
-Lemma leq_insert: forall t: tree, forall n n0: nat,
-  n <= n0 /\ all_leq n0 t -> all_leq n0 (insert n t).
-Proof.
-intros.
-destruct H.
-induction t.
-- simpl. auto.
-- simpl. simpl in H0.
-  destruct H0 as [H1 [H2 H3]].
-  destruct (n <=? n1) as []eqn:?.
-  * simpl; auto.
-  * simpl; auto.
-Defined.
-
-Lemma ge_insert: forall t: tree, forall n n0: nat,
-  n > n0 /\ all_geq n0 t -> all_geq n0 (insert n t).
-Proof.
-intros.
-destruct H.
-induction t.
-- simpl. auto.
-- simpl. simpl in H0.
-  destruct H0 as [H1 [H2 H3]].
-  destruct (n <=? n1) as []eqn:?.
-  * simpl; auto.
-  * simpl; auto.
-Defined.
-
-Lemma insert_correctness: forall t: tree, forall n: nat, bst t -> bst (insert n t).
-Proof.
-intros.
-induction t.
-* simpl; auto.
-* simpl; simpl in H.
-  destruct H as [H1 [H2 [H3 H4]]].
-  destruct (n <=? n0) as []eqn:?.
-  - simpl.
-    repeat split.
-    apply leq_insert.
-    split.
-    apply leb_complete in Heqb.
-    assumption.
-    assumption. 
-    assumption.
-    apply IHt1; assumption.
-    assumption.
-  - simpl.
-    apply leb_complete_conv in Heqb.
-    repeat split.
-    assumption.
-    apply ge_insert.
-    auto.
-    assumption.
-    apply IHt2; assumption.
-Defined.
-
-Compute(sort_insert [3;2;11] leaf).
+(*
 Compute(insert 2 (node leaf 3 leaf)).
+Compute(sort_insert [3;2;11]).
+Compute(insert 2 (node leaf 3 leaf)).
+Compute (treeMin (node (node leaf 11 leaf) 3 (node leaf 1 (node leaf 3 leaf)))).
 
-Lemma insertion_equality_forward: forall t1 t2: tree, forall a: nat,
-  t1 = t2 -> insert a t1 = insert a t2.
-Proof.
-intros.
-induction t1.
-- induction t2.
-  * reflexivity.
-  * rewrite H; reflexivity.
-- rewrite H; reflexivity.
-Defined.
+Compute(search (node (node leaf 2 leaf) 5 (node (node leaf 7 leaf) 8 leaf)) 5).
+Compute(search (node (node leaf 2 leaf) 5 (node (node leaf 7 leaf) 8 leaf)) 7).
+Compute(search (node (node leaf 2 leaf) 5 (node (node leaf 7 leaf) 8 leaf)) 11).
+Compute(search (node (node leaf 2 leaf) 5 (node (node leaf 7 leaf) 8 leaf)) 2).
+*)
+
+Section PartOneLemmas.
+
+(* 
+  This section contains:
+  n <= n0 /\ all_leq n0 t -> all_leq n0 (insert n t)
+  n > n0 /\ all_geq n0 t -> all_geq n0 (insert n t)
+  bst t -> bst (insert n t)
+  t1 = t2 -> insert a t1 = insert a t2
+  insert a t1 = insert a t2 -> t1 = t2 ---Incomplete
+  occurs a (insert a t)
+  a = n \/ occurs n t -> occurs n (insert a t)
+  occurs n (insert a t) -> a = n \/ occurs n t
+  
+*)
+Section InsertLemmas.
+  Lemma leq_insert: forall t: tree, forall n n0: nat,
+    n <= n0 /\ all_leq n0 t -> all_leq n0 (insert n t).
+  Proof.
+  intros.
+  destruct H.
+  induction t.
+  - simpl. auto.
+  - simpl. simpl in H0.
+    destruct H0 as [H1 [H2 H3]].
+    destruct (n <=? n1) as []eqn:?.
+    * simpl; auto.
+    * simpl; auto.
+  Qed.
+
+  Lemma gr_insert: forall t: tree, forall n n0: nat,
+    n > n0 /\ all_geq n0 t -> all_geq n0 (insert n t).
+  Proof.
+  intros.
+  destruct H.
+  induction t.
+  - simpl. auto.
+  - simpl. simpl in H0.
+    destruct H0 as [H1 [H2 H3]].
+    destruct (n <=? n1) as []eqn:?.
+    * simpl; auto.
+    * simpl; auto.
+  Qed.
+
+  Lemma insert_correctness: forall t: tree, forall n: nat, 
+    bst t -> bst (insert n t).
+  Proof.
+  intros.
+  induction t.
+  * simpl; auto.
+  * simpl; simpl in H.
+    destruct H as [H1 [H2 [H3 H4]]].
+    destruct (n <=? n0) as []eqn:?.
+    - simpl.
+      repeat split.
+      apply leq_insert.
+      split.
+      apply leb_complete in Heqb.
+      assumption.
+      assumption. 
+      assumption.
+      apply IHt1; assumption.
+      assumption.
+    - simpl.
+      apply leb_complete_conv in Heqb.
+      repeat split.
+      assumption.
+      apply gr_insert.
+      auto.
+      assumption.
+      apply IHt2; assumption.
+  Defined.
+
+  Lemma inserted_element_present: forall t: tree, forall a: nat,
+    occurs a (insert a t).
+  Proof.
+  intros.
+  induction t.
+  - simpl. auto.
+  - simpl.
+    destruct (a <=? n).
+    * simpl. right. left. assumption.
+    * simpl. right. right. assumption.
+  Defined.
+
+  Lemma insert_retains_elements: forall t: tree, forall a n: nat,
+     a = n \/ occurs n t -> occurs n (insert a t).
+  Proof.
+  intros.
+  destruct H.
+  - rewrite H.
+    apply inserted_element_present.
+  - induction t.
+    * simpl in H. simpl. auto.
+    * simpl.
+      simpl in H.
+      destruct H as [H1 | [H2 | H3]].
+      + destruct (a <=? n0).
+        simpl. auto.
+        simpl. auto.
+      + destruct (a <=? n0).
+        simpl. auto.
+        simpl. auto.
+      + destruct (a <=? n0).
+        simpl. auto.
+        simpl. auto.
+  Defined.
+
+  Lemma insert_retains_elements_back: forall t: tree, forall a n: nat,
+     occurs n (insert a t) -> a = n \/ occurs n t.
+  Proof.
+  intros.
+  induction t.
+  - simpl in H. destruct H as [H1|[H2|H3]]. auto. auto. auto.
+  - simpl in H.
+    destruct (a <=? n0).
+    * simpl in H.
+      simpl.
+      destruct H as [H1|[H2|H3]].
+      + auto.
+      + apply or_comm. apply or_assoc. right. 
+        apply or_assoc. apply or_comm. apply or_assoc. right.
+        auto.
+      + apply or_comm. apply or_assoc. right.
+        apply or_assoc. right.
+        auto.
+    * simpl.
+      simpl in H.
+      destruct H as [H1|[H2|H3]].
+      + auto.
+      + apply or_comm. apply or_assoc. right.
+        apply or_assoc. apply or_comm. apply or_assoc. right.
+        auto.
+      + apply or_comm. apply or_assoc. right.
+        apply or_assoc. right.
+        apply or_comm. auto.
+  Defined.
+End InsertLemmas.
+
+(*
+  This section contains:
+  occurs x t -> In x (to_list t
+  In x (to_list t) -> occurs x t
+*)
+Section ToListLemmas.
+  Lemma to_list_retains_elements: forall t: tree, forall x: nat,
+    occurs x t -> In x (to_list t).
+  Proof.
+  intros.
+  induction t.
+  - simpl. simpl in H. assumption.
+  - simpl in H.
+    destruct H.
+    * rewrite H.
+      simpl.
+      apply in_elt.
+    * destruct H.
+      + simpl.
+        apply in_or_app.
+        left; apply IHt1; assumption.
+      + simpl.
+        apply in_or_app.
+        right.
+        apply in_cons.
+        apply IHt2; assumption.
+  Defined.
+
+  Lemma to_list_retains_elements_back: forall t: tree, forall x: nat,
+    In x (to_list t) -> occurs x t.
+  Proof.
+  intros.
+  induction t.
+  - auto.
+  - simpl.
+    simpl in H.
+    apply in_app_or in H.
+    simpl.
+    destruct H as [H1|[H2|H3]].
+    * auto.
+    * left. auto.
+    * right. right. auto.
+  Defined.
+End ToListLemmas.
 
 
-Lemma insertion_equality: forall t1 t2: tree, forall a: nat,
-  insert a t1 = insert a t2 -> t1 = t2.
-Proof.
-intros.
-induction t1.
-- simpl in H.
-Admitted.
+(*
+  This section contains:
+  sort_insert (l1 ++ l2) t = sort_insert l1 (sort_insert l2 t)
+  bst t -> bst (sort_insert l t)
+  bst (sort t)
 
-Lemma sort_insert_append_assoc: forall l1 l2: (list nat), forall t: tree,
-  sort_insert (l1 ++ l2) t = sort_insert l1 (sort_insert l2 t).
-Proof.
-intros.
-induction l2.
-- simpl.
-  rewrite app_nil_r.
-  reflexivity.
-- simpl.
-  induction l1.
-  * simpl; reflexivity.
-  * simpl. simpl in IHl2.
-    rewrite IHl1.
-    reflexivity.
-    apply insertion_equality in IHl2.
+  In n l -> occurs n (sort_insert l leaf)
+  occurs n (sort_insert l leaf) -> In n l
+  occurs n t -> occurs n (sort t)
+  occurs n (sort t) -> occurs n t
+  occurs n t <-> occurs n (sort t)
+*)
+Section SortLemmas.
+
+  
+  Lemma sort_insert_is_bst: forall l: list nat,
+    bst (sort_insert l).
+  Proof.
+  intros.
+  induction l.
+  - simpl. tauto.
+  - simpl.
+    apply insert_correctness.
     assumption.
-Defined.
+  Defined.
 
+  Lemma sort_result_is_bst: forall t: tree, bst (sort t).
+  Proof.
+  intros.
+  unfold sort.
+  induction t.
+  - simpl. tauto.
+  - apply sort_insert_is_bst.
+  Qed.
 
-Lemma sort_insert_correctness: forall t: tree, forall l: (list nat),
-  bst t -> bst (sort_insert l t).
-Proof.
-intros.
-induction l.
-- auto.
-- simpl.
-  apply insert_correctness.
-  auto.
-Defined.
-
-Lemma sort_result_is_bst: forall t: tree, bst (sort t).
-Proof.
-intros.
-unfold sort.
-induction t.
-- simpl. tauto.
-- simpl.
-  rewrite sort_insert_append_assoc.
-  simpl.
-  apply sort_insert_correctness.
-  apply insert_correctness.
-  assumption.
-Qed.
-
-Lemma inserted_element_present: forall t: tree, forall a: nat,
-  occurs a (insert a t).
-Proof.
-intros.
-induction t.
-- simpl. auto.
-- simpl.
-  destruct (a <=? n).
-  * simpl. right. left. assumption.
-  * simpl. right. right. assumption.
-Defined.
-
-Lemma insert_retains_elements: forall t: tree, forall a n: nat,
-   a = n \/ occurs n t -> occurs n (insert a t).
-Proof.
-intros.
-destruct H.
-- rewrite H.
-  apply inserted_element_present.
-- induction t.
-  * simpl in H. simpl. auto.
-  * simpl.
+  Lemma sort_insert_retention: forall n: nat, forall l: (list nat),
+    In n l -> occurs n (sort_insert l).
+  Proof.
+  intros.
+  induction l.
+  - auto.
+  - simpl.
     simpl in H.
+    destruct H.
+    * apply insert_retains_elements.
+      auto.
+    * apply insert_retains_elements.
+      right. auto.
+  Defined.
+
+  Lemma sort_insert_retention_back: forall n: nat, forall l: (list nat),
+    occurs n (sort_insert l) -> In n l.
+  Proof.
+  intros.
+  induction l.
+  - auto.
+  - simpl.
+    simpl in H.
+    apply insert_retains_elements_back in H.
+    destruct H.
+    * auto.
+    * right.
+      auto.
+  Defined.
+
+  Lemma sort_retention_forward: forall n: nat, forall t: tree,
+    occurs n t -> occurs n (sort t).
+  Proof.
+  intros.
+  induction t.
+  - simpl; simpl in H; assumption.
+  - simpl in H.
+    apply sort_insert_retention.
     destruct H as [H1 | [H2 | H3]].
-    + destruct (a <=? n0).
-      simpl. auto.
-      simpl. auto.
-    + destruct (a <=? n0).
-      simpl. auto.
-      simpl. auto.
-    + destruct (a <=? n0).
-      simpl. auto.
-      simpl. auto.
-Defined.
-
-Print or_comm.
-
-Lemma insert_retains_elements_back: forall t: tree, forall a n: nat,
-   occurs n (insert a t) -> a = n \/ occurs n t .
-Proof.
-intros.
-induction t.
-- simpl in H. destruct H as [H1|[H2|H3]]. auto. auto. auto.
-- simpl in H.
-  destruct (a <=? n0).
-  * simpl in H.
-    simpl.
-    destruct H as [H1|[H2|H3]].
-    + auto.
-    + apply or_comm. apply or_assoc. right. 
-      apply or_assoc. apply or_comm. apply or_assoc. right.
-      auto.
-    + apply or_comm. apply or_assoc. right.
-      apply or_assoc. right.
-      auto.
-  * simpl.
-    simpl in H.
-    destruct H as [H1|[H2|H3]].
-    + auto.
-    + apply or_comm. apply or_assoc. right.
-      apply or_assoc. apply or_comm. apply or_assoc. right.
-      auto.
-    + apply or_comm. apply or_assoc. right.
-      apply or_assoc. right.
-      apply or_comm. auto.
-Defined.
-
-Lemma sort_insert_retention: forall n: nat, forall l: (list nat),
-  In n l -> occurs n (sort_insert l leaf).
-Proof.
-intros.
-induction l.
-- auto.
-- simpl.
-  simpl in H.
-  destruct H.
-  * apply insert_retains_elements.
-    auto.
-  * apply insert_retains_elements.
-    right. auto.
-Defined.
-
-Lemma sort_insert_retention_back: forall n: nat, forall l: (list nat),
-  occurs n (sort_insert l leaf) -> In n l.
-Proof.
-intros.
-induction l.
-- auto.
-- simpl.
-  simpl in H.
-  apply insert_retains_elements_back in H.
-  destruct H.
-  * auto.
-  * right.
-    auto.
-Defined.
-
-Lemma to_list_retains_elements: forall t: tree, forall x: nat,
-  occurs x t -> In x (to_list t).
-Proof.
-intros.
-induction t.
-- simpl. simpl in H. assumption.
-- simpl in H.
-  destruct H.
-  * rewrite H.
-    simpl.
-    apply in_elt.
-  * destruct H.
-    + simpl.
+    * simpl.
       apply in_or_app.
-      left; apply IHt1; assumption.
-    + simpl.
+      right.
+      rewrite H1.
+      apply in_eq.
+    * simpl.
+      apply in_or_app.
+      left.
+      apply to_list_retains_elements.
+      assumption.
+    * simpl.
       apply in_or_app.
       right.
       apply in_cons.
-      apply IHt2; assumption.
-Defined.
+      apply to_list_retains_elements.
+      assumption.
+  Defined.
 
-Lemma to_list_retains_elements_back: forall t: tree, forall x: nat,
-  In x (to_list t) -> occurs x t.
+  Lemma sort_retention_backward: forall n: nat, forall t: tree,
+     occurs n (sort t) -> occurs n t.
+  Proof.
+  intros.
+  induction t.
+  - simpl; simpl in H; assumption.
+  - simpl.
+    apply sort_insert_retention_back in H.
+    simpl in H.
+    apply in_app_or in H.
+    simpl in H.
+    destruct H as [H1 | [H2|H3]].
+    * right;left.
+      apply to_list_retains_elements_back.
+      auto.
+    * auto.
+    * right; right.
+      apply to_list_retains_elements_back.
+      auto.
+  Defined.
+
+  Lemma sort_retention: forall n: nat, forall t: tree,
+    occurs n t <-> occurs n (sort t).
+  Proof.
+  intros.
+  split.
+  apply sort_retention_forward.
+  apply sort_retention_backward.
+  Qed.
+
+End SortLemmas.
+
+End PartOneLemmas.
+
+Section PartTwoLemmas.
+
+Lemma min_element_in_tree: forall t: tree,
+  treeMin t <> None -> occurs_opt (treeMin t) t.
 Proof.
 intros.
-induction t.
-- auto.
-- simpl.
-  simpl in H.
-  apply in_app_or in H.
-  simpl.
-  destruct H as [H1|[H2|H3]].
-  * auto.
-  * left. auto.
-  * right. right. auto.
-Defined.
-
-
-Lemma occurs_retention_forward: forall n: nat, forall t: tree,
-  occurs n t -> occurs n (sort t).
-Proof.
-intros.
-induction t.
-- simpl; simpl in H; assumption.
-- simpl in H.
-  apply sort_insert_retention.
-  destruct H as [H1 | [H2 | H3]].
-  * simpl.
-    apply in_or_app.
-    right.
-    rewrite H1.
-    apply in_eq.
-  * simpl.
-    apply in_or_app.
-    left.
-    apply to_list_retains_elements.
-    assumption.
-  * simpl.
-    apply in_or_app.
-    right.
-    apply in_cons.
-    apply to_list_retains_elements.
-    assumption.
-Defined.
-
-Lemma occurs_retention_backward: forall n: nat, forall t: tree,
-   occurs n (sort t) -> occurs n t.
-Proof.
-intros.
-induction t.
-- simpl; simpl in H; assumption.
-- simpl.
-  apply sort_insert_retention_back in H.
-  simpl in H.
-  apply in_app_or in H.
-  simpl in H.
-  destruct H as [H1 | [H2|H3]].
-  * right;left.
-    apply to_list_retains_elements_back.
-    auto.
-  * auto.
-  * right; right.
-    apply to_list_retains_elements_back.
-    auto.
-Defined.
-
-Lemma occurs_retention: forall n: nat, forall t: tree,
-  occurs n t <-> occurs n (sort t).
-Proof.
-intros.
-split.
-apply occurs_retention_forward.
-apply occurs_retention_backward.
 Qed.
+End PartTwoLemmas.
